

Examples

De Morgan: $\neg(p \wedge q) \vdash (\neg p \vee \neg q)$.

Proof (dynamic mode):

1	$\neg(p \wedge q)$	
2	$\neg(\neg p \vee \neg q)$	
3	$\neg p$	
4	$(\neg p \vee \neg q)$	$\vee I \quad 3$
5	\perp	$\perp I \quad 2, 4$
6	$\neg\neg p$	$\neg I \quad 3 - 5$
7	p	$\neg E \quad 6$
8	$\neg q$	
9	$(\neg p \vee \neg q)$	$\vee I \quad 8$
10	\perp	$\perp I \quad 2, 9$
11	$\neg\neg q$	$\neg I \quad 8 - 10$
12	q	$\neg E \quad 11$
13	$(p \wedge q)$	$\wedge I \quad 7, 12$
14	\perp	$\perp I \quad 1, 13$
15	$\neg\neg(\neg p \vee \neg q)$	$\neg I \quad 2, 14$
16	$(\neg p \vee \neg q)$	$\neg E \quad 15$

Some Natural Deduction Rules

m	p	
n	q	
o	$(p \wedge q)$	$\wedge I \quad m, n$

m	$(p \wedge q)$	
n_1	p	$\wedge E \quad m$
n_2	q	$\wedge E \quad m$

m	p	
n	$(p \vee q)$	$\vee I \quad m$

a	$(p \vee q)$	
b	p	
c	r	
d	q	
e	r	
f	r	$\vee E \quad a, b - c, d - e$

Excluded Middle: $\vdash (p \vee \neg p)$

1	$\neg(p \vee \neg p)$	
2	p	
3	$(p \vee \neg p)$	$\vee I \quad 2$
4	\perp	$\perp I \quad 1, 3$
5	$\neg p$	$\neg I \quad 2 - 4$
6	$(p \vee \neg p)$	$\vee I \quad 5$
7	\perp	$\perp I \quad 1, 6$
8	$\neg\neg(p \vee \neg p)$	$\neg I \quad 1 - 7$
9	$p \vee \neg p$	$\neg E \quad 8$